deps/poulet4/lib/Monads/Transformers.v
@@ -1,4 +1,4 @@
-Require Export Poulet4.Monads.Monad Poulet4.Monads.State.
+Require Export Poulet4.Monads.Monad Poulet4.Monads.ExceptionState.
 
 (* TODO: it seems like exc could be implicit but in practice, it needs to be manually instantiated *)
 Definition lift_opt {Result State Exception : Type} (exc : Exception) (x: option Result) : @state_monad State Exception Result :=
