deps/poulet4/lib/P4light/Transformations/GenLoc.v
@@ -1,8 +1,7 @@
 Require Import Poulet4.P4light.Syntax.Syntax.
 From Poulet4.P4light.Syntax Require Import Typed SyntaxUtil.
 Require Import Poulet4.P4light.Transformations.SimplExpr.
-Require Import Poulet4.Monads.Monad.
-Require Import Poulet4.Monads.State.
+Require Import Poulet4.Monads.ExceptionState.
 Require Import Coq.Strings.String.
 Require Import Coq.Strings.Ascii.
 Require Import Coq.NArith.NArith.
